coqgen/coqgen.ml
@@ -31,7 +31,7 @@ let make_ml_type vars =
         None)
       (Path.Map.bindings vars.type_map)
   in
-  CTinductive { name = ml_type; args = []; kind = CTsort Set; cases }
+  CTinductive [{ name = ml_type; args = []; kind = CTsort Set; cases }]
 
 let make_subst = Coqtypes.make_subst ~mkcoq:mkcoqty ~mkml:(fun x -> x)
 
@@ -126,23 +126,70 @@ let make_compare_rec vars =
                      CTapp (CTid"M", [CTid "comparison"]))))
              )))
 
+let topo_sort (type def) (deps : def -> string * Names.t) (defs : def list) =
+  let edges = List.map deps defs in
+  let edge id1 id2 =
+    try Names.mem id2 (List.assoc id1 edges) with Not_found -> false in
+  let rec add (id : string) (dep : Names.t) (groups : string list list) =
+    match groups with
+      [] -> [[id]]
+    | gr :: rem ->
+        if List.exists (fun x -> Names.mem x dep) gr then
+          let cycle, groups' = get_cycle id groups in
+          (id :: cycle) :: groups'
+        else
+          gr :: add id dep rem
+  and get_cycle id = function
+      [] -> [], []
+    | gr :: rem as groups ->
+        let cycle, rem' = get_cycle id rem in
+        if cycle <> [] then gr @ cycle, rem' else
+        if List.exists (fun x -> edge x id) gr then gr, rem'
+        else [], groups
+  in
+  let groups =
+    List.fold_left (fun groups (id,dep) -> add id dep groups) [] edges in
+  let id_defs = List.combine (List.map fst edges) defs in
+  List.map (List.map (fun id -> List.assoc id id_defs)) groups
+
+let inductive_of_exn vars =
+  let constrs =
+    match Path.Map.find_opt Predef.path_exn vars.type_map with
+      Some {ct_coqdef = constrs} -> constrs
+    | _ -> assert false
+  in
+  let cases =
+    List.map
+      (fun (cstr, args) -> cstr, List.map (fun ct -> "_", ct) args, None)
+      constrs
+  in
+  CTinductive [{ name = "ml_exns"; args = []; kind = CTsort Type; cases }]
+
+let deps_inductive ind =
+  let types =
+    List.map snd ind.args @
+    List.flatten (List.map (fun (_, args, _) -> List.map snd args) ind.cases)
+  in
+  let vars = List.map coq_vars types in
+  (ind.name, List.fold_left Names.union Names.empty vars)
+
 let transl_implementation _modname st =
   let cmds, vars = transl_structure ~vars:init_vars st.str_items in
   let typedefs, cmds =
     List.partition (function CTinductive _ -> true | _ -> false) cmds
   in
-  (*let exceptions =
-    CTinductive
-      { name = "ml_exns"; kind = CTsort *)
+  let typedefs = typedefs @ [inductive_of_exn vars] in
+  let inductives =
+    List.flatten
+      (List.map (function CTinductive ind -> ind | _ -> assert false) typedefs)
+  in
+  let inductives = topo_sort deps_inductive inductives in
+  let typedefs = List.map (fun gr -> CTinductive gr) inductives in
+
   CTverbatim "From mathcomp Require Import ssreflect ssrnat seq.\
-\nRequire Import Int63 Ascii String Floats cocti_defs.\
+\nRequire Import Sint63 Ascii String Floats cocti_defs.\
 \n\n(* Generated representation of all ML types *)" ::
   make_ml_type vars ::
-  CTverbatim "\
-\nInductive ml_exns {M : Type -> Type} :=\
-\n  | Invalid_argument (_ : string)\
-\n  | Failure (_ : string)\
-\n  | Not_found.\n" ::
   CTverbatim "(* Module argument for monadic functor *)\
 \nModule MLtypes.\
 \nDefinition ml_type_eq_dec (T1 T2 : ml_type) : {T1=T2}+{T1<>T2}.\
@@ -160,7 +207,7 @@ let transl_implementation _modname st =
 \nVariant loc : ml_type -> Type := mkloc : forall k : key, loc (key_type k).\
 \n\
 \nSection with_monad.\
-\nVariable M : Type -> Type.\
+\nContext [M : Type -> Type].\
 \n\n(* Generated type definitions *)" ::
   typedefs @
   CTverbatim "Local (* Generated type translation function *)" ::
@@ -173,7 +220,7 @@ let transl_implementation _modname st =
 \nModule REFmonadML := REFmonad (MLtypes).\
 \nExport REFmonadML.\
 \n\
-\nDefinition coq_type := MLtypes.coq_type M.\
+\nDefinition coq_type := @MLtypes.coq_type M.\
 \nDefinition empty_env := mkEnv 0%int63 nil.\
 \nDefinition it : W unit := (empty_env, inl tt).\
 \n\n(* Generated comparison function *)" ::
