coqgen/coqtypes.mli
@@ -35,11 +35,16 @@ val find_instantiation :
   vars:coq_env ->
   coq_term_desc -> type_expr -> coq_term list
 
-val transl_typedecl :
-    loc:Location.t ->
-    env:Env.t ->
-    vars:coq_env ->
-    Ident.t -> type_declaration -> vernacular * coq_env
+val transl_typedecls :
+  env:Env.t ->
+  vars:coq_env ->
+  Typedtree.type_declaration list -> vernacular * coq_env
+
+val transl_exception :
+  loc:Location.t ->
+  env:Env.t ->
+  vars:coq_env ->
+  Typedtree.extension_constructor -> coq_env
 
 val close_type : type_expr -> unit
 
