testsuite/tests/coqgen/test2.ml
@@ -1,0 +1,40 @@
+(* Some more tests *)
+
+type t = E of exn
+
+exception T of t
+
+type t0 = O | T1 of t1
+and t1 = T2 of t2
+and t2 = T0 of t0
+
+let x = T0 O;;
+
+T2 x;;
+
+let failwith s = raise (Failure s);;
+
+let rec length_aux len = function
+    [] -> len
+  | _::l -> length_aux (len + 1) l
+
+let length l = length_aux 0 l
+
+let cons a l = a::l
+
+let hd = function
+    [] -> failwith "hd"
+  | a::_ -> a
+
+(*type student = { name: string; mutable year: int }
+
+Record student_val := { name: string; year: int }.
+Definition student := loc student_val.
+
+type _ tag = Int : int tag | Bool : bool tag
+
+let rec f : type a. a tag -> bool list -> a = fun tag l ->
+  match tag with
+  | Int -> 3
+  | Bool -> true
+*)
