testsuite/tests/coqgen/test2.v
@@ -1,0 +1,204 @@
+From mathcomp Require Import ssreflect ssrnat seq.
+Require Import Sint63 Ascii String Floats cocti_defs.
+
+(* Generated representation of all ML types *)
+Inductive ml_type :=
+  | ml_int
+  | ml_char
+  | ml_float
+  | ml_bool
+  | ml_unit
+  | ml_exn
+  | ml_array (_ : ml_type)
+  | ml_list (_ : ml_type)
+  | ml_string
+  | ml_empty
+  | ml_array_t (_ : ml_type)
+  | ml_t
+  | ml_t0
+  | ml_t1
+  | ml_t2
+  | ml_ref (_ : ml_type)
+  | ml_arrow (_ : ml_type) (_ : ml_type).
+
+(* Module argument for monadic functor *)
+Module MLtypes.
+Definition ml_type_eq_dec (T1 T2 : ml_type) : {T1=T2}+{T1<>T2}.
+revert T2; induction T1; destruct T2;
+  try (right; intro; discriminate); try (now left);
+  try (case (IHT1_5 T2_5); [|right; injection; intros; contradiction]);
+  try (case (IHT1_4 T2_4); [|right; injection; intros; contradiction]);
+  try (case (IHT1_3 T2_3); [|right; injection; intros; contradiction]);
+  try (case (IHT1_2 T2_2); [|right; injection; intros; contradiction]);
+  (case (IHT1 T2) || case (IHT1_1 T2_1)); try (left; now subst);
+    right; injection; intros; contradiction.
+Defined.
+
+Local Definition ml_type := ml_type.
+Record key := mkkey {key_id : int; key_type : ml_type}.
+Variant loc : ml_type -> Type := mkloc : forall k : key, loc (key_type k).
+
+Section with_monad.
+Context [M : Type -> Type].
+
+(* Generated type definitions *)
+Inductive ml_exns :=
+  | T (_ : t)
+  | Invalid_argument (_ : string)
+  | Failure (_ : string)
+  | Not_found
+with t := E (_ : ml_exns).
+
+Inductive t2 := T0 (_ : t0)
+with t0 := | O | T1_1 (_ : t1)
+with t1 := T2_1 (_ : t2).
+
+Local (* Generated type translation function *)
+Fixpoint coq_type (T : ml_type) : Type :=
+  match T with
+  | ml_int => Int63.int
+  | ml_char => Ascii.ascii
+  | ml_float => float
+  | ml_bool => bool
+  | ml_unit => unit
+  | ml_exn => ml_exns
+  | ml_array T1 => loc (ml_array_t T1)
+  | ml_list T1 => list (coq_type T1)
+  | ml_string => String.string
+  | ml_empty => empty
+  | ml_array_t T1 => array_t (coq_type T1)
+  | ml_t => t
+  | ml_t0 => t0
+  | ml_t1 => t1
+  | ml_t2 => t2
+  | ml_ref T1 => loc T1
+  | ml_arrow T1 T2 => coq_type T1 -> M (coq_type T2)
+  end.
+
+End with_monad.
+Local Definition ml_exn := ml_exn.
+End MLtypes.
+Export MLtypes.
+
+Module REFmonadML := REFmonad (MLtypes).
+Export REFmonadML.
+
+Definition coq_type := @MLtypes.coq_type M.
+Definition empty_env := mkEnv 0%int63 nil.
+Definition it : W unit := (empty_env, inl tt).
+
+(* Generated comparison function *)
+Fixpoint compare_rec (h : nat) (T : ml_type)
+  : coq_type T -> coq_type T -> M comparison :=
+  if h is h.+1 then
+    let compare_rec := compare_rec h in
+    match T as T return coq_type T -> coq_type T -> M comparison with
+    | ml_int => fun x y => Ret (Sint63.compare x y)
+    | ml_char => fun x y => Ret (compare_ascii x y)
+    | ml_float => fun x y => Ret (compare_float x y)
+    | ml_bool => fun x y => Ret (Bool.compare x y)
+    | ml_unit => fun x y => Ret Eq
+    | ml_exn =>
+      fun x y =>
+        match x, y with
+        | Not_found, Not_found => Ret Eq
+        | T x1, T y1 => compare_rec ml_t x1 y1
+        | Invalid_argument x1, Invalid_argument y1 =>
+          compare_rec ml_string x1 y1
+        | Failure x1, Failure y1 => compare_rec ml_string x1 y1
+        | Not_found, _ => Ret Lt
+        | _, Not_found => Ret Gt
+        | T _, _ => Ret Lt
+        | _, T _ => Ret Gt
+        | Invalid_argument _, _ => Ret Lt
+        | _, Invalid_argument _ => Ret Gt
+        end
+    | ml_array T1 => fun x y => compare_ref compare_rec (ml_array_t T1) x y
+    | ml_list T1 => fun x y => compare_list compare_rec T1 x y
+    | ml_string => fun x y => Ret (compare_string x y)
+    | ml_empty => fun x y => match x with end
+    | ml_array_t T1 =>
+      fun x y =>
+        match x, y with
+        | ArrayVal x1, ArrayVal y1 => compare_rec (ml_list T1) x1 y1
+        end
+    | ml_t =>
+      fun x y => match x, y with | E x1, E y1 => compare_rec ml_exn x1 y1 end
+    | ml_t0 =>
+      fun x y =>
+        match x, y with
+        | O, O => Ret Eq
+        | T1_1 x1, T1_1 y1 => compare_rec ml_t1 x1 y1
+        | O, _ => Ret Lt
+        | _, O => Ret Gt
+        end
+    | ml_t1 =>
+      fun x y =>
+        match x, y with | T2_1 x1, T2_1 y1 => compare_rec ml_t2 x1 y1 end
+    | ml_t2 =>
+      fun x y =>
+        match x, y with | T0 x1, T0 y1 => compare_rec ml_t0 x1 y1 end
+    | ml_ref T1 => fun x y => compare_ref compare_rec T1 x y
+    | ml_arrow T1 T2 =>
+      fun x y => Fail (Catchable (Invalid_argument "compare"%string))
+    end
+  else fun _ _ => FailGas.
+
+Definition ml_compare := compare_rec.
+
+Definition wrap_compare wrap T h x y : M bool :=
+  do c <- compare_rec T h x y; Ret (wrap c).
+
+Definition ml_eq := wrap_compare (fun c => if c is Eq then true else false).
+Definition ml_lt := wrap_compare (fun c => if c is Lt then true else false).
+Definition ml_gt := wrap_compare (fun c => if c is Gt then true else false).
+Definition ml_ne := wrap_compare (fun c => if c is Eq then false else true).
+Definition ml_ge := wrap_compare (fun c => if c is Lt then false else true).
+Definition ml_le := wrap_compare (fun c => if c is Gt then false else true).
+
+(* Array operations *)
+Definition newarray T len (x : coq_type T) :=
+  do len <- nat_of_int len; newref (ml_array_t T) (ArrayVal _ (nseq len x)).
+Definition getarray T (a : coq_type (ml_array T)) n : M (coq_type T) :=
+  do s <- getref (ml_array_t T) a;
+  let: ArrayVal s := s in
+  do n <- bounded_nat_of_int (seq.size s) n;
+  if s is x :: _ then Ret (nth x s n) else
+  raise _ (Invalid_argument "getarray").
+Definition setarray T (a : coq_type (ml_array T)) n (x : coq_type T) :=
+  do s <- getref (ml_array_t T) a;
+  let: ArrayVal s := s in
+  do n <- bounded_nat_of_int (seq.size s) n;
+  setref (ml_array_t T) a (ArrayVal _ (set_nth x s n x)).
+
+(* Default amount of gas *)
+Definition h := 100000.
+
+(* Translated code *)
+
+Definition x := T0 O.
+
+Eval vm_compute in T2_1 x.
+
+Definition failwith (T_1 : ml_type) (s : coq_type ml_string)
+  : M (coq_type T_1) := raise T_1 (Failure s).
+
+Fixpoint length_aux (h : nat) (T_1 : ml_type) (len : coq_type ml_int)
+  (param : coq_type (ml_list T_1)) : M (coq_type ml_int) :=
+  if h is h.+1 then
+    match param with
+    | @nil _ => Ret len
+    | _ :: l => length_aux h T_1 (Int63.add len 1%int63) l
+    end
+  else FailGas.
+
+Definition length (h : nat) (T_1 : ml_type) (l : coq_type (ml_list T_1))
+  : M (coq_type ml_int) := length_aux h T_1 0%int63 l.
+
+Definition cons_1 (T_1 : ml_type) (a : coq_type T_1)
+  (l : coq_type (ml_list T_1)) : coq_type (ml_list T_1) := a :: l.
+
+Definition hd (T_1 : ml_type) (param : coq_type (ml_list T_1))
+  : M (coq_type T_1) :=
+  match param with | @nil _ => failwith T_1 "hd"%string | a :: _ => Ret a end.
+
